theories/TrainingComputations/interp_max_utils.v
@@ -1,0 +1,83 @@
+From Coq Require Import Derive.
+From Coq.Structures Require Import Equalities.
+From Coq Require Import PreOmega Zify Lia ZifyUint63 Sint63 Floats Uint63 ZArith NArith.
+From NeuralNetInterp.Util Require Import PrimitiveProd.
+From NeuralNetInterp.Util.Tactics Require Import IsUint63 ChangeInAll ClearAll BreakMatch.
+From NeuralNetInterp.Util Require Export Default Pointed.
+From NeuralNetInterp.Util Require Import Wf_Uint63.
+From NeuralNetInterp.Util.Arith Require Import Classes Instances.
+From NeuralNetInterp.Torch Require Import Tensor Slicing Tensor.Proofs Tensor.Instances.
+From NeuralNetInterp.TransformerLens Require Import HookedTransformer HookedTransformer.Config HookedTransformer.Module.
+Import Instances.Truncating Instances.Uint63.
+#[local] Open Scope tensor_scope.
+#[local] Open Scope core_scope.
+
+Module ModelComputations (cfg : Config) (Import Model : ModelSig cfg).
+  Import (hints) cfg.
+  Import Optimize.
+
+  Section generic.
+    Context {A} {coer_float : has_coer float A} {coerZ : has_coer Z A}
+      {addA : has_add A} {subA : has_sub A} {mulA : has_mul A} {divA : has_div A}
+      {sqrtA : has_sqrt A} {expA : has_exp A}
+      {maxA : has_max A} {minA : has_min A}
+      {use_checkpoint : with_default "use_checkpoint" bool true}
+      (defaultA : pointed A := @coer _ _ coerZ point).
+    Let coerA' (x : float) : A := coer x.
+    #[local] Coercion coerA' : float >-> A.
+    #[local] Existing Instance defaultA.
+
+    Definition logit_delta : A
+      := let all_tokens
+           := PArray.maybe_checkpoint all_tokens in
+         let all_predicted_logits : tensor [_;_;_] A
+           := PArray.maybe_checkpoint (Model.HookedTransformer.logits all_tokens) in
+         let predicted_logits : tensor [_;_] A
+           := all_predicted_logits.[:,-1,:] in
+         let indices_of_max : tensor [_;1] RawIndexType
+           := Tensor.max_dim_m1 (keepdim:=true) all_tokens in
+         let correct_logits
+           := gather_dim_m1 predicted_logits indices_of_max in
+         let logits_above_correct
+           := PArray.maybe_checkpoint (correct_logits - predicted_logits) in
+         let bigger_than_anything : A
+           := Tensor.item (Tensor.max logits_above_correct) in
+         let logits_above_correct : tensor [cfg.d_vocab ^ cfg.n_ctx : N; cfg.n_ctx] A
+           := fun '(((tt, b), i) as idxs)
+              => if i =? Tensor.item indices_of_max.[b,0]
+                 then bigger_than_anything
+                 else Tensor.item logits_above_correct.[b,i] in
+         let min_incorrect_logit
+           := Tensor.min_dim_m1 logits_above_correct in
+         Tensor.item (Tensor.min min_incorrect_logit).
+  End generic.
+
+  Definition logit_delta_float : float := logit_delta.
+(*
+  Derive logit_delta_float_opt
+    SuchThat (logit_delta_float_opt = logit_delta_float)
+    As logit_delta_float_opt_eq.
+  Proof.
+    start_optimizing ().
+    cbv beta iota delta [logit_delta].
+    do_red ().
+    red_early_layers (); red_late_layers_1 (); red_late_layers_2 ().
+    cbv beta zeta in *; do_red (); subst_local_cleanup ().
+    set (logits := HookedTransformer.logits _) in all_predicted_logits.
+    assert (PArray.abstract logits_all_tokens_concrete_opt = logits).
+    rewrite logits_all_tokens_concrete_opt_eq.
+    cbv [logits logits_all_tokens_concrete].
+    Search PArray.concretize.
+
+    cbv [] in *.
+    cbn [fst snd Shape.tl Shape.hd] in *.
+    red_ops ().
+    do_red ().
+
+    cbv [logits
+    revert_lets_eq ().
+    finish_optimizing ().
+  Qed.
+  Definition logit_delta_
+ *)
+End ModelComputations.
